src/AbstractDomain.v
@@ -17,6 +17,7 @@ Class adom (concrete_state abstract_state: eqType) :=
     le_trans: forall a1 a2 a3, le a1 a2 -> le a2 a3 -> le a1 a3;
     gamma_monotone : forall a1 a2, le a1 a2 <-> Included concrete_state (gamma a1) (gamma a2);
     gamma_top : forall x, Ensembles.In concrete_state (gamma top) x;
+    gamma_bot : forall x, ~ Ensembles.In concrete_state (gamma bot) x;
     join_spec : forall a1 a2 x, Ensembles.In concrete_state (gamma (join a1 a2)) x <->
                          Ensembles.In concrete_state (gamma a1) x \/
                          Ensembles.In concrete_state (gamma a2) x;
